sandbox/BohmTrees.v
@@ -1,0 +1,224 @@
+(** * Bohm Trees *)
+
+Require Import Coq.Program.Basics.
+Require Import Coq.Program.Equality.
+Require Import Coq.Logic.Decidable.
+Require Import Coq.Bool.Bool.
+Require Import DeBruijn.
+
+(** Bohm trees generalize the normal forms of pure lambda-calculus,
+    where the language is extended by
+    a term [BOT],
+    a reduction rule [BOT x -beta-> BOT],
+    and an approximation rule [x -pi-> BOT].
+
+    In the lambda-join-calculus, we also have
+    terms [JOIN x y],
+    a reduction rule [JOIN x y * z -beta-> JOIN (x * z) (y * z)],
+    and three approximation rules:
+    [x -pi-> z -> y -pi-z> -> JOIN x y -pi-> z],
+    [JOIN x y -pi-> x], and
+    [JOIN x y -pi-> y].
+    We also add an identifiable top term [TOP] with
+    a reduction rule [TOP x -beta-> TOP],
+    and an approximation rule [TOP -pi-> x].
+    *)
+
+Inductive normal {Var : Set} : Term Var -> Prop :=
+  | normal_top : normal TOP
+  | normal_bot : normal BOT
+  | normal_join x y : normal x -> normal y -> normal (x || y)
+  | normal_rand x y : normal x -> normal y -> normal (x (+) y)
+  | normal_app x y : inert x -> normal y -> normal (x * y)
+  | normal_lambda x : @normal (option Var) x -> normal (LAMBDA x)
+  | normal_var v : normal (VAR v)
+with inert {Var : Set} : Term Var -> Prop :=
+  | inert_var v : inert (VAR v)
+  | inert_app x y : inert x -> normal y -> inert (x * y)
+.
+Hint Constructors normal inert.
+
+Lemma inert_normal {Var : Set} (x : Term Var) : inert x -> normal x.
+Proof.
+  intro H; induction H; eauto.
+Qed.
+
+Fixpoint is_normal {Var : Set} (w : Term Var) {struct w} : bool :=
+  match w with
+  | TOP => true
+  | BOT => true
+  | x || y => andb (is_normal x) (is_normal y)
+  | x (+) y => andb (is_normal x) (is_normal y)
+  | x * y => andb (is_inert x) (is_normal y)
+  | LAMBDA x => is_normal x
+  | VAR v => true
+  end
+with is_inert {Var : Set} (w : Term Var) {struct w} : bool :=
+  match w with
+  | x * y => andb (is_inert x) (is_normal y)
+  | VAR v => true
+  | _ => false
+  end.
+
+Lemma is_inert_is_normal {Var : Set} (x : Term Var) :
+  is_inert x = true -> is_normal x = true.
+Proof.
+  induction x; simpl; auto; intro H; inversion H.
+Qed.
+
+Lemma normal_is_normal {Var : Set} (x : Term Var) :
+  normal x <-> is_normal x = true.
+(* normal x <-> eq_true (is_normal x) *)
+(* normal x <-> is_true (is_normal x) *)
+(* normal x <-> Is_true (is_normal x) *)
+Proof.
+  split.
+  - intro H; induction H; simpl; auto.
+    + rewrite IHnormal1; rewrite IHnormal2; simpl; auto.
+    + rewrite IHnormal1; rewrite IHnormal2; simpl; auto.
+    + rewrite IHnormal; simpl; auto.
+      admit.
+  - dependent induction x; simpl; intros; eauto.
+    + revert H;
+      (* FIXME need to simultaneously do induction on inert and normal
+      case_eq (is_inert x1); case_eq (is_normal x2); simpl;
+      intros Ex2 Ex1 H; destruct H; auto.
+      apply is_inert_is_normal in Ex1.
+      rewrite Ex1 in IHx1; rewrite Ex2 in IHx2; simpl.
+      *)
+      admit.
+    + admit.
+    + admit.
+Qed.
+
+Lemma normal_decidable {Var : Set} (x : Term Var) : decidable (normal x).
+Proof.
+  unfold decidable; rewrite normal_is_normal; decide equality.
+Qed.
+
+Fixpoint try_reduce_step {Var : Set} (x : Term Var) : option (Term Var) :=
+  match x with
+  | TOP * y => Some TOP
+  | BOT * y => Some BOT
+  | (x1 || x2) * y => Some (x1 * y || x2 * y)
+  | (x1 (+) x2) * y => Some (x1 * y (+) x2 * y)
+  | LAMBDA x1 * x2 => Some (beta_sub x1 x2)
+  | l * r =>
+      match try_reduce_step l with
+      | Some l' => Some (l' * r)
+      | None =>
+          match try_reduce_step r with
+          | Some r' => Some (l * r')
+          | None => None
+          end
+      end
+  | (l || r) =>
+      match try_reduce_step l with
+      | Some l' => Some (l' || r)
+      | None =>
+          match try_reduce_step r with
+          | Some r' => Some (l || r')
+          | None => None
+          end
+      end
+  | l (+) r =>
+      match try_reduce_step l with
+      | Some l' => Some (l' (+) r)
+      | None =>
+          match try_reduce_step r with
+          | Some r' => Some (l (+) r')
+          | None => None
+          end
+      end
+  | LAMBDA y => 
+      match try_reduce_step y with
+      | Some y' => Some (LAMBDA y')
+      | None => None
+      end
+  | _ => None
+  end.
+
+Fixpoint is_irreducible {Var : Set} (x : Term Var) : bool :=
+  match x with
+  | TOP * _ => false
+  | BOT * _ => false
+  | (_ || _) * _ => false
+  | (_ (+) _) * _ => false
+  | LAMBDA x1 * x2 => false
+  | l * r => andb (is_irreducible l) (is_irreducible r)
+  | l || r => andb (is_irreducible l) (is_irreducible r)
+  | l (+) r => andb (is_irreducible l) (is_irreducible r)
+  | LAMBDA x1 => is_irreducible x1
+  | _ => true
+  end.
+
+Definition is_none {a : Set} (x : option a) : bool :=
+  match x with
+  | None => true
+  | Some _ => false
+  end.
+
+Local Ltac case_some x H :=
+  let x' := fresh x "'" in
+  let Hx' := fresh x "'" in
+  intros x' Hx';
+  rewrite Hx' in H; simpl in H; rewrite H;
+  simpl.
+
+Local Ltac case_none x H :=
+  let Hx' := fresh x "'" in
+  intro Hx';
+  rewrite Hx' in H; simpl in H; rewrite H;
+  simpl.
+
+Local Ltac cases_option x IHx :=
+  case_eq (try_reduce_step x); [case_some x IHx | case_none x IHx].
+
+Local Ltac cases_option2 x1 x2 IHx1 IHx2 :=
+  cases_option x1 IHx1;
+  [ case x1; auto
+  | cases_option x2 IHx2; case x1; auto
+  ].
+
+Lemma try_reduce_step_is_irreducible {Var : Set} (x : Term Var) :
+  is_irreducible x = is_none (try_reduce_step x).
+Proof.
+  induction x; simpl; auto.
+  - cases_option2 x1 x2 IHx1 IHx2.
+  - cases_option2 x1 x2 IHx1 IHx2.
+  - cases_option2 x1 x2 IHx1 IHx2.
+  - cases_option x IHx; auto.
+Qed.
+
+Theorem is_irreducible_is_normal {Var : Set} (x : Term Var) :
+  is_irreducible x = is_normal x.
+Proof.
+  induction x; simpl; auto.
+  - rewrite IHx1; rewrite IHx2; clear IHx1 IHx2; revert x2.
+    induction x1; simpl; auto.
+  - rewrite IHx1; rewrite IHx2; clear IHx1 IHx2; simpl.
+    case (is_normal x1); case (is_normal x2); simpl; reflexivity.
+  - rewrite IHx1; rewrite IHx2; clear IHx1 IHx2; simpl.
+    induction x1; auto.
+Qed.
+
+(** Many properties of Bohm trees are decidable *)
+
+Fixpoint normal_conv {Var : Set} (x : Term Var) : normal x -> bool.
+Admitted.
+
+Inductive dyadic : Set :=
+  | dyadic_one : dyadic
+  | dyadic_zero : dyadic
+  | dyadic_rand : dyadic -> dyadic -> dyadic.
+
+Fixpoint normal_pconv {Var : Set} (x : Term Var) : normal x -> dyadic.
+Admitted.
+
+Fixpoint normal_is_le {Var : Set} (x y : Term Var) :
+  normal x -> normal y -> bool.
+Admitted.
+
+Definition normal_is_eq
+  {Var : Set} (x y : Term Var) (nx : normal x) (ny : normal y) : bool :=
+  andb (normal_is_le x y nx ny) (normal_is_le y x ny nx).
